Test/dafny0/ExternConstraints.dfy
@@ -10,6 +10,28 @@ module {:extern "Mod"} Mod1
 
   class {:extern "classx"} Class1
   {
-    method {:extern "method1"} method1(obj: MyClass, x: int) requires x >= 0
+    method {:extern} method1(obj: MyClass, x: int) requires x >= 0
+    
+    method {:extern} method2(obj: MyClass, x: int) requires x >= 0
+    {
+      
+    }
+    
+    method {:extern} method3(obj: MyClass?, x: int)
+    {
+      if (x >= 0 && obj != null) {
+        method2(obj, x);
+      }
+    }
+    
+    method {:extern} method4(context: map<object?, string>)
+    {
+
+    }
+
+    method {:extern} method5(foo: int)
+    {
+
+    }
   }
 }
